src/CSL/Leased_Heap.v
@@ -1,0 +1,209 @@
+From iris.algebra Require Import auth gmap frac agree namespace_map excl.
+From stdpp Require Export namespaces.
+From iris.base_logic.lib Require Export own.
+From iris.base_logic.lib Require Import gen_heap.
+From iris.bi.lib Require Import fractional.
+From iris.proofmode Require Import tactics.
+Set Default Proof Using "Type".
+Import uPred.
+
+Class leased_heapG (L V : Type) (Σ : gFunctors) `{Countable L} := LeasedHeapG {
+  leased_heap_heapG :> gen_heapG L V Σ;
+  leased_heap_exclG :> inG Σ (authR (optionUR (exclR (leibnizC V))));
+  leased_heap_gen : namespace;
+}.
+Arguments leased_heap_heapG {_ _ _ _ _} _ : assert.
+Arguments leased_heap_exclG {_ _ _ _ _} _ : assert.
+Arguments leased_heap_gen {_ _ _ _ _} _ : assert.
+
+Class leased_heapPreG (L V : Type) (Σ : gFunctors) `{Countable L} := {
+  leased_heap_heapPreG :> gen_heapPreG L V Σ;
+  leased_heap_exclPreG :> inG Σ (authR (optionUR (exclR (leibnizC V))));
+}.
+
+Definition leased_heapΣ (L V : Type) `{Countable L} : gFunctors := #[
+  gen_heapΣ L V; GFunctor (authR (optionUR (exclR (leibnizC V))))
+].
+
+Instance subG_leased_heapPreG {Σ L V} `{Countable L} :
+  subG (leased_heapΣ L V) Σ → leased_heapPreG L V Σ.
+Proof. solve_inG. Qed.
+
+Definition current_gen (N: namespace) := ndot N 0.
+Definition next_gen (N: namespace) := ndot N 1.
+
+Lemma split_gen_disj N : current_gen N ## next_gen N.
+Proof. solve_ndisj. Qed.
+
+Definition next_leased_heapG `{hG: leased_heapG L V Σ} :=
+  LeasedHeapG _ _ _ _ _ (@leased_heap_heapG _ _ _ _ _ hG)
+                        (@leased_heap_exclG _ _ _ _ _ hG)
+                        (next_gen (leased_heap_gen hG)).
+
+Section definitions.
+  Context {L V} `{Countable L, hG: !leased_heapG L V Σ}.
+
+  Definition lease (l: L) (v : V) :=
+    (∃ γ : gname, meta l (current_gen (leased_heap_gen hG)) γ
+                  ∗ own γ (◯ (Excl' (v: leibnizC V))))%I.
+
+  (* TODO: alternate name possibilities: 'deed' or 'title'? *)
+  Definition master (l: L) (v: V) :=
+    (∃ γ : gname, meta l (current_gen (leased_heap_gen hG)) γ
+                  ∗ meta_token l (↑ next_gen (leased_heap_gen hG))
+                  ∗ own γ (● (Excl' (v: leibnizC V))))%I.
+End definitions.
+
+Local Notation "l ↦{ q } v" := (mapsto l q v)
+  (at level 20, q at level 50, format "l  ↦{ q }  v") : bi_scope.
+Local Notation "l ↦ v" := (mapsto l 1 v) (at level 20) : bi_scope.
+
+Local Notation "l ↦{ q } -" := (∃ v, l ↦{q} v)%I
+  (at level 20, q at level 50, format "l  ↦{ q }  -") : bi_scope.
+Local Notation "l ↦ -" := (l ↦{1} -)%I (at level 20) : bi_scope.
+
+Definition next_lease `{hG: leased_heapG L V Σ} (l: L) (v : V) :=
+  lease (hG := next_leased_heapG) l v.
+
+Definition next_master `{hG: leased_heapG L V Σ} (l: L) (v : V) :=
+  master (hG := next_leased_heapG) l v.
+
+
+Section lease_heap.
+  Context {L V} `{Countable L, hG: !leased_heapG L V Σ}.
+
+  Implicit Types P Q : iProp Σ.
+  Implicit Types Φ : V → iProp Σ.
+  Implicit Types σ : gmap L V.
+  Implicit Types m : gmap L gname.
+  Implicit Types h g : gen_heapUR L V.
+  Implicit Types l : L.
+  Implicit Types v : V.
+
+  (** General properties of leases and masters *)
+  Global Instance lease_timeless l v : Timeless (lease l v).
+  Proof. apply _. Qed.
+  Global Instance master_timeless l v : Timeless (master l v).
+  Proof. apply _. Qed.
+
+  Lemma master_lease_agree l (v1 v2 : V) :
+    master l v1 -∗ lease l v2 -∗ ⌜v1 = v2⌝.
+  Proof.
+    iDestruct 1 as (γm1) "(Hγ1&_&Hown1)"; iDestruct 1 as (γm2) "(Hγ2&Hown2)".
+    iDestruct (meta_agree with "Hγ1 Hγ2") as %->.
+    iDestruct (own_valid_2 with "Hown1 Hown2") as "H".
+    iDestruct "H" as %[<-%Excl_included%leibniz_equiv _]%auth_both_valid.
+    done.
+  Qed.
+
+  Lemma meta_lease_init N l (γ: gname):
+    meta_token l (↑N) ==∗ meta l (current_gen N) γ ∗ meta_token l (↑ next_gen N).
+  Proof.
+    rewrite (union_difference_L (↑ next_gen N) (↑N)); last by solve_ndisj.
+    iIntros "H".
+    iDestruct (meta_token_union with "H") as "($&?)"; first set_solver.
+    by iMod (meta_set _ _ γ (current_gen N) with "[$]") as "$"; first solve_ndisj.
+  Qed.
+
+  Lemma master_next l v :
+    master l v ==∗ next_master l v ∗ next_lease l v.
+  Proof.
+    iDestruct 1 as (γ) "(Hγ&Hrest&Hown)".
+    iMod (own_alloc (● (Excl' (v: leibnizC V)) ⋅ ◯ (Excl' (v: leibnizC V)))) as (γ') "[H1 H2]".
+    { apply auth_both_valid; split; eauto. econstructor. }
+    iMod (meta_lease_init _ _ γ' with "Hrest") as "(#Hset&Hrest)".
+    iModIntro. iSplitL "Hrest H1"; by iExists _; iFrame.
+  Qed.
+
+  Lemma master_lease_alloc l v :
+    meta_token l ⊤ ==∗ master l v ∗ lease l v.
+  Proof.
+    iIntros "H".
+    iMod (own_alloc (● (Excl' (v: leibnizC V)) ⋅ ◯ (Excl' (v: leibnizC V)))) as (γ) "[H1 H2]".
+    { apply auth_both_valid; split; eauto. econstructor. }
+    rewrite (union_difference_L (↑ leased_heap_gen hG) ⊤); last by solve_ndisj.
+    iDestruct (meta_token_union with "H") as "(H&_)"; first set_solver.
+    iMod (meta_lease_init _ _ γ with "H") as "(#Hset&Hrest)".
+    iModIntro. iSplitL "Hrest H1"; by iExists _; iFrame.
+  Qed.
+
+  Lemma big_sepM_master_lease_alloc σ :
+    ([∗ map] l↦v ∈ σ, meta_token l ⊤) ==∗ ([∗ map] l↦v ∈ σ, master l v ∗ lease l v).
+  Proof.
+    iIntros "H".
+    iApply (big_opM_forall (λ P Q, P ==∗ Q)); auto using bupd_intro.
+    { intros P1 P2 HP Q1 Q2 HQ. by rewrite HP HQ -bupd_sep. }
+    iApply big_sepM_mono; last by eauto.
+    intros; by iApply master_lease_alloc.
+  Qed.
+
+  Lemma master_lease_update l v v0 v':
+    master l v -∗ lease l v0 ==∗ master l v' ∗ lease l v'.
+  Proof.
+    iDestruct 1 as (γm1) "(Hγ1&Hrest&Hown1)"; iDestruct 1 as (γm2) "(Hγ2&Hown2)".
+    iDestruct (meta_agree with "Hγ1 Hγ2") as %->.
+    iMod (own_update_2 _ _ _ (● Excl' (v': leibnizC V) ⋅ ◯ Excl' (v': leibnizC V))
+            with "Hown1 Hown2") as "[Hown1 Hown2]".
+    { by apply auth_update, option_local_update, exclusive_local_update. }
+    iModIntro.
+    iSplitL "Hγ1 Hrest Hown1"; iExists _; iFrame.
+  Qed.
+
+  Lemma leased_heap_alloc σ l v :
+    σ !! l = None →
+    gen_heap_ctx σ ==∗ gen_heap_ctx (<[l:=v]>σ) ∗ l ↦ v ∗ master l v ∗ lease l v.
+  Proof.
+    iIntros (Hσl) "H".
+    iMod (gen_heap_alloc σ l v with "H") as "($&$&H)"; first done.
+    by iApply master_lease_alloc.
+  Qed.
+
+End lease_heap.
+
+Lemma heap_init_to_bigOp `{hG: leased_heapG L V Σ} (σ: gmap L V):
+  own (i := @gen_heap_inG _ _ _ _ _ (leased_heap_heapG hG))
+      (gen_heap_name (leased_heap_heapG hG))
+      (◯ to_gen_heap σ)
+      -∗
+  [∗ map] i↦v ∈ σ,  i ↦ v .
+Proof.
+  induction σ as [| ???? IH] using map_ind.
+  - iIntros. rewrite //=.
+  - iIntros "Hown".
+    rewrite big_opM_insert //.
+
+    iAssert (own (i := @gen_heap_inG _ _ _ _ _ (leased_heap_heapG hG))
+                 (gen_heap_name (leased_heap_heapG hG))
+                 (◯ to_gen_heap m) ∗
+                 (i ↦ x))%I
+                    with "[Hown]" as "[Hrest $]".
+    {
+      rewrite mapsto_eq /mapsto_def //.
+      rewrite to_gen_heap_insert insert_singleton_op; last by apply lookup_to_gen_heap_None.
+      rewrite auth_frag_op. iDestruct "Hown" as "(?&?)". iFrame.
+    }
+    by iApply IH.
+Qed.
+
+Lemma leased_heap_strong_init `{H: leased_heapPreG L V Σ} σ :
+  (|==> ∃ (H0 : leased_heapG L V Σ)
+          (Hpf: @gen_heap_inG _ _ _ _ _ (leased_heap_heapG H0) =
+                gen_heap_preG_inG), gen_heap_ctx σ
+                ∗ ([∗ map] i↦v ∈ σ, i ↦ v ∗ master i v ∗ lease i v))%I.
+Proof.
+  iMod (own_alloc (● to_gen_heap ∅)) as (γ) "Hg".
+  { rewrite auth_auth_valid. exact: to_gen_heap_valid. }
+  iMod (own_alloc (● to_gen_meta ∅)) as (γm) "Hm".
+  { rewrite auth_auth_valid. exact: to_gen_meta_valid. }
+  set (hG := (GenHeapG L V Σ _ _ _ _ _ γ γm)).
+  set (hL := (LeasedHeapG L V Σ _ _ hG _ (1%positive :: nil))).
+  iAssert (gen_heap_ctx (hG := hG) ∅) with "[-]" as "H".
+  { iExists ∅. iFrame. eauto. }
+  iMod (gen_heap_alloc_gen ∅ σ with "H") as "(Hctx&Hheap&Hmeta)".
+  { apply map_disjoint_empty_r. }
+  rewrite right_id_L.
+  iMod (big_sepM_master_lease_alloc σ with "Hmeta").
+  iModIntro.
+  iExists hL, eq_refl.
+  iFrame. iApply big_sepM_sep. iFrame.
+Qed.
