src/Examples/ExMach/Adequacy.v
@@ -1,5 +1,6 @@
 From iris.algebra Require Import auth gmap frac agree.
 Require Export CSL.WeakestPre CSL.Lifting CSL.Adequacy CSL.RefinementAdequacy CSL.RefinementIdempotenceFunModule.
+Require Export CSL.Leased_Heap.
 From iris.algebra Require Export functions.
 From iris.base_logic.lib Require Export invariants gen_heap.
 From iris.proofmode Require Export tactics.
@@ -8,11 +9,11 @@ Require Export ExMach.ExMachAPI ExMach.WeakestPre.
 Class exmachPreG Σ := ExMachPreG {
   exm_preG_iris :> invPreG Σ;
   exm_preG_mem :> gen_heapPreG nat nat Σ;
-  exm_preG_disk :> gen_heapPreG nat nat Σ;
+  exm_preG_disk :> leased_heapPreG nat nat Σ;
   exm_preG_treg_inG :> inG Σ (csumR countingR (authR (optionUR (exclR unitC))));
 }.
 
-Definition exmachΣ : gFunctors := #[invΣ; gen_heapΣ nat nat; gen_heapΣ nat nat;
+Definition exmachΣ : gFunctors := #[invΣ; gen_heapΣ nat nat; leased_heapΣ nat nat;
                                     GFunctor (csumR countingR (authR (optionUR (exclR unitC))))].
 Instance subG_exmachPreG {Σ} : subG exmachΣ Σ → exmachPreG Σ.
 Proof. solve_inG. Qed.
